-- {-# OPTIONS --allow-unsolved-metas #-}
module Lambda where

open import Logic
open import Lifting

-- Lambda terms as a type constructor
-- For a set X, Î› X = terms whose free variables come from the set X
-- Î› is \GL
data Î› (V : Set) : Set where
  var : V â†’ Î› V
  app : Î› V â†’ Î› V â†’ Î› V
  abs : Î› (â†‘ V) â†’ Î› V

-- Terms over a finite set of variables, Î›á¶  n = Î› {x1, ..., xn}
-- á¶  is \^f
Î›á¶  : â„• â†’ Set
Î›á¶  n = Î› (Fin n)

-- The set of closed terms, whose set of free variables is empty
-- â° is \^0
Î›â° : Set
Î›â° = Î›á¶  0 -- Î› âŠ¥

-- Functorial action on morphisms
Î›â†’ : âˆ€ {A B : Set} (f : A â†’ B) â†’ Î› A â†’ Î› B
Î›â†’ f (var x)   = var (f x)
Î›â†’ f (app s t) = app (Î›â†’ f s) (Î›â†’ f t)
Î›â†’ f (abs r)   = abs (Î›â†’ (â†‘â†’ f) r)

-- A very common special case
Î›â†’i : âˆ€ {A : Set} â†’ Î› A â†’ Î› (â†‘ A)
Î›â†’i = Î›â†’ i

-- Preservation of pointwise equality
Î›â†’â‰… : âˆ€ {A B : Set} {f g : A â†’ B} â†’ f â‰… g â†’ Î›â†’ f â‰… Î›â†’ g
Î›â†’â‰… fg (var x)   = cong  var (fg x)
Î›â†’â‰… fg (app s t) = cong2 app (Î›â†’â‰… fg s) (Î›â†’â‰… fg t)
Î›â†’â‰… fg (abs r)   = cong  abs (Î›â†’â‰… (â†‘â†’â‰… fg) r)

-- Preservation of identity
Î›â†’â‰…I : âˆ€ {A} {f : A â†’ A} â†’ f â‰… I â†’ Î›â†’ f â‰… I
Î›â†’â‰…I fâ‰…I (var x)   = cong  var (fâ‰…I x)
Î›â†’â‰…I fâ‰…I (app s t) = cong2 app (Î›â†’â‰…I fâ‰…I s) (Î›â†’â‰…I fâ‰…I t)
Î›â†’â‰…I fâ‰…I (abs r)   = cong  abs (Î›â†’â‰…I (â†‘â†’â‰…I fâ‰…I) r)

-- Preservation of composition
Î›â†’âˆ˜ : âˆ€ {A B C} (f : A â†’ B) (g : B â†’ C) â†’ Î›â†’ (g âˆ˜ f) â‰… Î›â†’ g âˆ˜ Î›â†’ f
Î›â†’âˆ˜ f g (var x)   = refl
Î›â†’âˆ˜ f g (app s t) = cong2 app (Î›â†’âˆ˜ f g s) (Î›â†’âˆ˜ f g t)
Î›â†’âˆ˜ f g (abs r)   = cong  abs (Î›â†’â‰… (â†‘â†’âˆ˜ f g) r ! Î›â†’âˆ˜ (â†‘â†’ f) (â†‘â†’ g) r)

-- Preservation of composition modulo pointwise equality
-- The Original Version
-- (This lemma looks more complicated, but its proof is simpler than the above)
Î›â†’â‰…âˆ˜ : âˆ€ {A B C} (f : A â†’ B) (g : B â†’ C) {h} â†’ h â‰… g âˆ˜ f â†’ Î›â†’ h â‰… Î›â†’ g âˆ˜ Î›â†’ f
-- Î›â†’â‰…âˆ˜ f g hâ‰…gâˆ˜f = Î›â†’â‰… hâ‰…gâˆ˜f â‰…!â‰… Î›â†’âˆ˜ f g
Î›â†’â‰…âˆ˜ f g hâ‰…gâˆ˜f (var x)   = cong  var (hâ‰…gâˆ˜f x)
Î›â†’â‰…âˆ˜ f g hâ‰…gâˆ˜f (app s t) = cong2 app (Î›â†’â‰…âˆ˜ f g hâ‰…gâˆ˜f s) (Î›â†’â‰…âˆ˜ f g hâ‰…gâˆ˜f t)
Î›â†’â‰…âˆ˜ f g hâ‰…gâˆ˜f (abs r)   = cong  abs (Î›â†’â‰…âˆ˜ (â†‘â†’ f) (â†‘â†’ g) (â†‘â†’â‰…âˆ˜ f g hâ‰…gâˆ˜f) r )

-- Preservation of composition modulo pointwise equality
-- Symmetric version
Î›â†’âˆ˜â‰… : âˆ€ {A B C} (f : A â†’ B) (g : B â†’ C) {h} â†’ g âˆ˜ f â‰… h â†’ Î›â†’ g âˆ˜ Î›â†’ f â‰… Î›â†’ h
-- Î›â†’âˆ˜â‰… f g gfâ‰…h = Î›â†’âˆ˜ f g ~!â‰… Î›â†’â‰… gfâ‰…h
Î›â†’âˆ˜â‰… f g gfâ‰…h (var x)     = cong  var (gfâ‰…h x)
Î›â†’âˆ˜â‰… f g gfâ‰…h (app t1 t2) = cong2 app (Î›â†’âˆ˜â‰… f g gfâ‰…h t1) (Î›â†’âˆ˜â‰… f g gfâ‰…h t2)
Î›â†’âˆ˜â‰… f g gfâ‰…h (abs t0)    = cong  abs (Î›â†’âˆ˜â‰… (â†‘â†’ f) (â†‘â†’ g) (â†‘â†’âˆ˜â‰… f g gfâ‰…h) t0)

-- Lifting a function over the type of terms
lift : âˆ€ {A B : Set} â†’ (A â†’ Î› B) â†’ â†‘ A â†’ Î› (â†‘ B)
lift f = io (Î›â†’i âˆ˜ f) (var o)

-- Lifting preserves pointwise equality
liftâ‰… : âˆ€ {A B : Set} {f g : A â†’ Î› B} â†’ f â‰… g â†’ lift f â‰… lift g
liftâ‰… fâ‰…g (i x) = cong Î›â†’i (fâ‰…g x)
liftâ‰… fâ‰…g o     = refl
-- liftâ‰… fâ‰…g = ioğ“Ÿ _ (Î» x â†’ cong Î›â†’i (fâ‰…g x)) refl

liftâ‰…âˆ˜ : âˆ€ {A B C} {f : A â†’ B} {g : B â†’ Î› C} {h} â†’ h â‰… g âˆ˜ f â†’ lift h â‰… lift g âˆ˜ â†‘â†’ f
liftâ‰…âˆ˜ hâ‰…gf (i x) = cong Î›â†’i (hâ‰…gf x)
liftâ‰…âˆ˜ hâ‰…gf o = refl

-- Substitution is the monadic bind for Î› (Haskell's >>=)
_[_] : âˆ€ {A B : Set} â†’ Î› A â†’ (A â†’ Î› B) â†’ Î› B
var x   [ f ] = f x
app s t [ f ] = app (s [ f ]) (t [ f ])
abs r   [ f ] = abs (r [ lift f ])

-- A special case of the above for finitely many variables
_[_]á¶  : âˆ€ {m n : â„•} â†’ Î›á¶  m â†’ (Fin m â†’ Î›á¶  n) â†’ Î›á¶  n
_[_]á¶  = _[_]

_[_]áµ’ : âˆ€ {X : Set} â†’ Î› (â†‘ X) â†’ Î› X â†’ Î› X
M [ N ]áµ’  = M [ io var N ]

bind : âˆ€ {A B : Set} â†’ (A â†’ Î› B) â†’ Î› A â†’ Î› B
bind f t = t [ f ]

bindâ‰… : âˆ€ {A B : Set} {f g : A â†’ Î› B} â†’ f â‰… g â†’ bind f â‰… bind g
bindâ‰… fâ‰…g (var x)     = fâ‰…g x
bindâ‰… fâ‰…g (app t1 t2) = cong2 app (bindâ‰… fâ‰…g t1 ) (bindâ‰… fâ‰…g t2)
bindâ‰… fâ‰…g (abs t0)    = cong abs (bindâ‰… (liftâ‰… fâ‰…g) t0)

bind-natâ‚ : âˆ€ {X Y Z : Set} {f : X â†’ Y} {g : Y â†’ Î› Z} {h}
              â†’ h â‰… g âˆ˜ f â†’ bind h â‰… bind g âˆ˜ Î›â†’ f
bind-natâ‚ hâ‰…gf (var x)     = hâ‰…gf x
bind-natâ‚ hâ‰…gf (app t1 t2) = cong2 app (bind-natâ‚ hâ‰…gf t1) (bind-natâ‚ hâ‰…gf t2)
bind-natâ‚ hâ‰…gf (abs t0)    = cong abs (bind-natâ‚ (liftâ‰…âˆ˜ hâ‰…gf) t0 )

bind-nat : âˆ€ {X Y : Set} (g : X â†’ Î› Y) â†’ Î›â†’ i âˆ˜ bind g â‰… bind (lift g) âˆ˜ Î›â†’ i
bind-nat g (var x)     = refl
bind-nat g (app t1 t2) = cong2 app (bind-nat g t1) (bind-nat g t2)
bind-nat g (abs t0)    = cong abs {! bind-nat (lift g)  t0  !}

bind-assocâ‰… : âˆ€ {A B C : Set} {f : A â†’ Î› B} {g : B â†’ Î› C} {h : A â†’ Î› C}
               â†’ h â‰… bind g âˆ˜ f â†’ bind h â‰… bind g âˆ˜ bind f
bind-assocâ‰… bgâˆ˜fâ‰…h (var x)     = bgâˆ˜fâ‰…h x
bind-assocâ‰… bgâˆ˜fâ‰…h (app t1 t2) = cong2 app (bind-assocâ‰… bgâˆ˜fâ‰…h t1) (bind-assocâ‰… bgâˆ˜fâ‰…h t2)
bind-assocâ‰… {f = f} {g} {h} bgâˆ˜fâ‰…h (abs t0)    = cong abs (bind-assocâ‰… eq t0) where
  eq = liftâ‰…âˆ˜ bgâˆ˜fâ‰…h â‰…!â‰… Î» {  (i x) â†’ {! liftâ‰…âˆ˜   !} ; o â†’ refl }
  -- eq = liftâ‰… bgâˆ˜fâ‰…h â‰…!â‰… Î» { (i x) â†’ bind-nat g (f x) ; o â†’ refl }
  -- ih = {!   !} -- Î» x â†’ {! Î›â†’â‰…âˆ˜ _ _ (symmâ‰… bgâˆ˜fâ‰…h) x    !}
  -- eq = ioğ“Ÿ (Î» a â†’ bind (lift g) (lift f a) â‰¡ lift h a) ih refl
-- bind-assocâ‰… {f = f} {g} bgâˆ˜fâ‰…h (abs t0) = cong abs (bind-assocâ‰… eq t0)
--   where eq : _ -- bind (lift g) âˆ˜ lift f â‰… lift h
--         eq (i x) = ~ (bind-nat g (f x)) ! (cong (Î›â†’ i) (bgâˆ˜fâ‰…h x))
--         eq o = refl

bind-assoc : âˆ€ {A B C : Set} {f : A â†’ Î› B} {g : B â†’ Î› C}
               â†’ bind (bind g âˆ˜ f) â‰… bind g âˆ˜ bind f
bind-assoc {f = f} {g} = bind-assocâ‰… reflâ‰…
-- bind-assoc {A} {B} {C} {f} {g} (var x) = refl
-- bind-assoc {A} {B} {C} {f} {g} (app t1 t2) = cong2 app (bind-assoc t1) (bind-assoc t2)
-- bind-assoc {A} {B} {C} {f} {g} (abs t0)
--   = cong abs {! bind-assoc t0   !}


-- The End
